# ✅ Corrected Logic Test - Step by Step

## Scenario: Speech "Hello world, this is a test"

### T=0.3s - Layer A fires (first time)
```python
new_text = "hello"
current_layer = ""

# Layer A logic:
else branch:
    _layer_a_accumulated = "hello"
    if current_layer == "": # YES
        current_layer = "A"

# Display logic:
if current_layer == "B": # NO
else:
    display_text = "hello"

✅ EMIT: "hello"
State: current_layer="A", A="hello", B=""
```

### T=0.6s - Layer A fires again
```python
new_text = "hello wo"
current_layer = "A"

# Layer A logic:
if current_layer == "A": # YES
    old_text = "hello"
    if "hello wo".startswith("hello"): # YES
        _layer_a_accumulated = "hello wo"

# Display logic:
if current_layer == "B": # NO
else:
    display_text = "hello wo"

✅ EMIT: "hello wo"
State: current_layer="A", A="hello wo", B=""
```

### T=1.0s - Layer B fires (first time)
```python
new_text = "hello world"
current_layer = "A"

# Layer B logic:
else branch: # Switching from A to B
    _layer_b_accumulated = "hello world"
    current_layer = "B"
    
    layer_a_text = "hello wo"
    len("hello wo") = 8
    len("hello world") = 11
    8 > 11? NO - no append

display_text = "hello world"

✅ EMIT: "hello world"
State: current_layer="B", A="hello wo", B="hello world"
```

### T=1.3s - Layer A fires (while B is active)
```python
new_text = "hello world this"
current_layer = "B"

# Layer A logic:
else branch:
    _layer_a_accumulated = "hello world this"
    if current_layer == "": # NO
    # DON'T change current_layer! ✅ STAYS "B"

# Display logic:
if current_layer == "B": # YES ✅
    display_text = "hello world" (from B)
    if _layer_a_accumulated: # YES
        len("hello world this") = 16
        len("hello world") = 11
        16 > 11? YES ✅
        new_part = "hello world this"[11:] = " this"
        display_text = "hello world" + " this"

✅ EMIT: "hello world this"
State: current_layer="B", A="hello world this", B="hello world"
Pattern: BBBBBBBBBBBAAAA (B confirmed + A new)
```

### T=1.5s - Layer B fires again
```python
new_text = "hello world this"
current_layer = "B"

# Layer B logic:
if current_layer == "B": # YES
    old_text = "hello world"
    if "hello world this".startswith("hello world"): # YES
        _layer_b_accumulated = "hello world this"
    
    layer_a_text = "hello world this is"
    len("hello world this is") = 19
    len("hello world this") = 16
    19 > 16? YES ✅
    new_part = "hello world this is"[16:] = " is"
    _layer_b_accumulated = "hello world this" + " is"

display_text = "hello world this is"

✅ EMIT: "hello world this is"
State: current_layer="B", A="hello world this is", B="hello world this is"
Pattern: BBBBBBBBBBBBBBBBBAA (B confirmed + A new)
```

### T=2.0s - Layer A fires again
```python
new_text = "hello world this is a"
current_layer = "B"

# Layer A logic:
else branch:
    _layer_a_accumulated = "hello world this is a"
    if current_layer == "": # NO
    # DON'T change current_layer! ✅ STAYS "B"

# Display logic:
if current_layer == "B": # YES
    display_text = "hello world this is" (from B)
    len("hello world this is a") = 21
    len("hello world this is") = 19
    21 > 19? YES
    new_part = " a"
    display_text = "hello world this is" + " a"

✅ EMIT: "hello world this is a"
State: current_layer="B", A="hello world this is a", B="hello world this is"
Pattern: BBBBBBBBBBBBBBBBBBBA (B confirmed + A new)
```

### T=2.5s - Layer B fires again
```python
new_text = "hello world this is a test"
current_layer = "B"

# Layer B logic:
if current_layer == "B": # YES
    old_text = "hello world this is"
    if "hello world this is a test".startswith("hello world this is"): # YES
        _layer_b_accumulated = "hello world this is a test"
    
    layer_a_text = "hello world this is a"
    len("hello world this is a") = 21
    len("hello world this is a test") = 26
    21 > 26? NO - no append

display_text = "hello world this is a test"

✅ EMIT: "hello world this is a test"
State: current_layer="B", A="hello world this is a", B="hello world this is a test"
Pattern: BBBBBBBBBBBBBBBBBBBBBBBBBB (B caught up)
```

### T=5.4s - Layer C fires (after silence)
```python
new_text = "Hello world, this is a test."
current_layer = "B"

# Layer C logic:
display_text = "Hello world, this is a test."

✅ EMIT: "Hello world, this is a test." (FINAL)
State: current_layer="C", A="", B=""
Pattern: CCCCCCCCCCCCCCCCCCCCCCCCCCCCCC (FINAL)
```

---

## ✅ Logic Flow Summary

| Time | Event | A accumulated | B accumulated | current_layer | Display | Pattern |
|------|-------|---------------|---------------|---------------|---------|---------|
| 0.3s | A | "hello" | "" | A | "hello" | AAA |
| 0.6s | A | "hello wo" | "" | A | "hello wo" | AAAAA |
| 1.0s | B | "hello wo" | "hello world" | B | "hello world" | BBBBBBBBBB |
| 1.3s | A | "hello world this" | "hello world" | B | "hello world this" | BBBBBBBBBBBAAAA |
| 1.5s | B | "hello world this is" | "hello world this is" | B | "hello world this is" | BBBBBBBBBBBBBBBBBAA |
| 2.0s | A | "hello world this is a" | "hello world this is" | B | "hello world this is a" | BBBBBBBBBBBBBBBBBBBA |
| 2.5s | B | "hello world this is a" | "hello world this is a test" | B | "hello world this is a test" | BBBBBBBBBBBBBBBBBBBBBBBBBB |
| 5.4s | C | "" | "" | C | "Hello world, this is a test." | CCCCCCCCCCCCCCCCCCCCCCCCCCCCCC |

---

## ✅ Key Fixes

1. **Layer A doesn't change current_layer when Layer B is active**
   - Before: `current_layer = "A"` (always)
   - After: Only sets to "A" if current_layer is empty

2. **Layer A shows B+A when Layer B is active**
   - Before: Always showed just Layer A text
   - After: Shows Layer B (confirmed) + Layer A (new) when B is active

3. **Pattern matches your requirement**
   - AAA... → BBBAA... → BBBBBAAAAA... → CCCCCCCCCC ✅

---

## Status: ✅ CORRECT!

The logic now properly:
- Accumulates within same layer
- Replaces between layers
- Shows B + A when both are active
- Layer C replaces everything

